src/3d/Options.fst
@@ -35,6 +35,7 @@ let output_dir : ref (option vstring) = alloc None
 let save_hashes : ref bool = alloc false
 let skip_makefiles : ref bool = alloc false
 let skip_deps: ref bool = alloc false
+let skip_o_rules: ref bool = alloc false
 
 let valid_micro_step (str: string) : Tot bool = match str with
   | "verify"
@@ -290,6 +291,7 @@ let (display_usage_2, compute_options_2, fstar_options) =
     CmdOption "odir" (OptStringOption "output directory" always_valid output_dir) "output directory (default '.'); writes <module_name>.fst and <module_name>_wrapper.c to the output directory" [];
     CmdOption "save_hashes" (OptBool save_hashes) "Save hashes" [];
     CmdOption "skip_makefiles" (OptBool skip_makefiles) "Do not Generate Makefile.basic, Makefile.include" [];
+    CmdOption "skip_o_rules" (OptBool skip_o_rules) "With --makefile, do not generate rules for .o files" [];
     CmdFStarOption (let open FStar.Getopt in noshort, "version", ZeroArgs (fun _ -> FStar.IO.print_string (Printf.sprintf "EverParse/3d %s\nCopyright 2018, 2019, 2020 Microsoft Corporation\n" Version.everparse_version); exit 0), "Show this version of EverParse");
     CmdOption "equate_types" (OptList "an argument of the form A,B, to generate asserts of the form (A.t == B.t)" valid_equate_types equate_types_list) "Takes an argument of the form A,B and then for each entrypoint definition in B, it generates an assert (A.t == B.t) in the B.Types file, useful when refactoring specs, you can provide multiple equate_types on the command line" [];
     CmdOption "__arg0" (OptStringOption "executable name" always_valid arg0) "executable name to use for the help message" [];
@@ -408,3 +410,6 @@ let get_makefile_name _ =
   match !makefile_name with
   | None -> OS.concat (get_output_dir ()) "EverParse.Makefile"
   | Some mf -> mf
+
+let get_skip_o_rules _ =
+  !skip_o_rules
