src/3d/GenMakefile.fsti
@@ -1,5 +1,6 @@
 module GenMakefile
 
 val write_gnu_makefile
+  (skip_o_rules: bool)
   (files: list string)
 : FStar.All.ML unit
